theories/check.v
@@ -24,9 +24,10 @@ Proof.
   rewrite incl_refl//.
 Qed.
 
-Lemma expand_det_tree {u sP sV sV' A r s ign d} : 
+Lemma expand_det_tree {u sP sV sVx sV' A r s ign d} : 
   check_program sP ->
-    sigma2ctx sP s = Some sV ->
+    sigma2ctx sP s = Some sVx ->
+      more_precise sVx sV ->
       tc_tree_aux sP sV A ign = ty_ok (d, sV') ->
         step u s A = r ->
           exists S d', minD d d' = d' /\ 
@@ -35,70 +36,91 @@ Lemma expand_det_tree {u sP sV sV' A r s ign d} :
 Proof.
   simpl in *.
   move=> CKPR.
-  move: sV sV' r d ign.
+  move: sV sV' sVx r d ign.
   pattern u, s, A, (step u s A).
   apply: expand_ind; clear -CKPR.
-  - move=> s []//= _ ???? _ _ [_ ->] <-/=; repeat eexists; rewrite ?minD_refl//.
-  - move=> s []//= _ ???? _ _ [_ ->] <-/=; repeat eexists; rewrite ?minD_refl//.
-  - move=> s []//= _ ???? _ _ [_ ->] <-/=; repeat eexists; rewrite ?minD_refl//.
+  - move=> s []//= _ ?????? _ _ [_ ->] <-/=; repeat eexists; rewrite ?minD_refl//.
+  - move=> s []//= _ ?????? _ _ [_ ->] <-/=; repeat eexists; rewrite ?minD_refl//.
+  - move=> s []//= _ ?????? _ _ [_ ->] <-/=; repeat eexists; rewrite ?minD_refl//.
   - (*here the checker comes into the game*)
-    move=> /=s A pr t HA sV1 sV2 r d ign + + <-/=; clear -CKPR.
+    move=> /=s A pr t HA sV1 sV2 sVx r d ign + + + <-/=; clear -CKPR.
     {
+      move=> H1 H2.
       rewrite/big_or.
       case X: F => /=[|[sr1 r1] rs]/=.
       - repeat eexists; rewrite minD_refl//.
-      - case C: check_callable => //=[[D SIG]].
+      - case C: check_callable => //=[[D SIG]][??]; subst.
         move: C; rewrite /check_callable.
         case C: check_tm => //=[[[S B]|]]//=; last first.
-          move=> [??] + [??]; subst.
-          rewrite maxD_comm/=.
-
-          (* call to unkown variable *)
+          rewrite/get_callable_hd_sig/get_tm_hd_sig.
+          case HD: get_tm_hd => //=[E|[P|V]]; [by destruct t|..].
+            case LP: lookup => //=[VP|]; last first.
+              move=> [??]; subst; rewrite maxD_comm/=.
+              (* a big_or always produces a tc valid tree  *)
+              admit.
+            case A: assume_call => //=[V] [??]; subst; rewrite maxD_comm//=.
+              (* a big_or always produces a tc valid tree  *)
+            admit.
+          case LP: lookup => //=[VP|]; last first.
+            move=> [??]; subst; rewrite maxD_comm/=.
+              (* a big_or always produces a tc valid tree  *)
+            admit.
+          case A: assume_call => //=[V'] [??]; subst; rewrite maxD_comm//=.
+          (* a big_or always produces a tc valid tree  *)
           admit.
-        move=> ++[??]; subst.
         case: S C => //=-[]//= d1.
         case: B; last first.
           (* miscall *)
           move=> + [??]; subst.
           rewrite maxD_comm/=.
+          (* a big_or always produces a tc valid tree  *)
           admit.
-        case G: get_callable_hd_sig => [hd|]; last first.
-          move=> +[??]; subst.
-          rewrite maxD_comm/=.
+        (* THIS A GOOD CALL!! *)
+        move=> H.
+        have : exists T d0, get_callable_hd_sig sP sV1 t = Some T /\ 
+          get_sig_hd T = d d0 /\ minD d0 d1 = d0.
           admit.
-        case ASS: assume_call => //=[SEND] + [??]; subst.
+        move=> [S[d0 [H3 [H4 H5]]]].
+        rewrite H3/=.
+        case ASS: assume_call => //=[SEND] [??]; subst.
         rewrite maxD_comm -maxD_assoc maxD_refl.
         destruct d1 => //=; last first.
+          (* a big_or always produces a tc valid tree  *)
           admit.
+        destruct ign => //=; last first.
+          (* a big_or always produces a tc valid tree  *)
+          admit.
+        (* !!! THIS IS THE TRULY INTERESTING CASE !!! *)
+        destruct d0; subst => //=.
         admit.
     }
-  - move=> s []//= _ ???? _ _ [_ ->] <-/=; repeat eexists; rewrite ?minD_refl//.
-    (* apply: sV_expand_refl. *)
-  - move=> s INIT A sB B HINIT dA IH sV sV' r d ign H/=.
+  - move=> s []//= _ ?????? _ _ [_ ->] <-/=; repeat eexists; rewrite ?minD_refl//.
+  - move=> s INIT A sB B HINIT dA IH sV sV' sVx r d ign H/= MP.
     rewrite is_dead_is_ko//=.
     have ?: sB = s by admit.
     subst.
     move=> tcA <-/=.
     rewrite get_tree_Or /= is_dead_is_ko//.
     apply: IH; eauto.
-  - move=> s INIT A sB B HINIT dA IH A' eA sV sV' r d ign H/=.
+  - move=> s INIT A sB B HINIT dA IH A' eA sV sV' sVx r d ign H/= MP.
     case: ifP => kA.
       by rewrite is_ko_step in eA.
     case: ifP => kB.
       move=> dtA <-{r}/=.
       rewrite kB.
-      have {IH}/=[S[d'[H1 H2]]]:= IH _ _ _ _ _ H dtA eA.
+      have {IH}/=[S[d'[H1 H2]]]:= IH _ _ _ _ _ _ H MP dtA eA.
       rewrite H2.
       rewrite is_ko_tc_tree_aux//=?(sigma2ctx_valid H)//.
       case: ifP; repeat eexists; auto.
       rewrite minD_refl//.
+      admit.
     have fA:= expand_not_failed _ eA notF.
     move=> + <-{r}/=.
     (* case nB: next_alt => [B'|]//=. *)
     case dtA: (tc_tree_aux _ _ A) => /=[[DA' sVA]|]//=.
     case dtB: (tc_tree_aux _ _ B) => /=[[DB sVB]|]//=.
     case M: merge_sig => //=[S']; subst.
-    have {IH}/=[S[d'[H1 H2]]]:= IH _ _ _ _ _ H dtA eA.
+    have {IH}/=[S[d'[H1 H2]]]:= IH _ _ _ _ _ _ H MP dtA eA.
     move=> [??]; subst.
     case kA' : (is_ko A'); last first.
       rewrite (expand_Exp_has_cut eA).
@@ -122,20 +144,20 @@ Proof.
     move=> /=.
     have:= same_ty_tc_tree_aux sP sV B ign Pred.
     rewrite dtB; case dtB': tc_tree_aux => //=[[D1 S1]]; repeat eexists.
-  - move=> s INIT A sB B HINIT dA IH A' eA sV sV' r d ign H/=.
+  - move=> s INIT A sB B HINIT dA IH A' eA sV sV' sVx r d ign H/= MP.
     case: ifP => kA.
       by rewrite is_ko_step in eA.
     case: ifP => kB.
       move=> dtA <-/=.
       rewrite (expand_CB_is_ko eA) is_ko_cutr.
-      have /=[S[d'[H1 H2]]] := IH _ _ _ _ _ H dtA eA.
+      have /=[S[d'[H1 H2]]] := IH _ _ _ _ _ _ H MP dtA eA.
       by rewrite H2; repeat eexists.
     have fA:= expand_not_failed _ eA notF.
     case dtA: (tc_tree_aux _ _ A) => /=[[DA' sVA]|]//=.
     case dtB: (tc_tree_aux _ _ B) => /=[[DB sVB]|]//=.
     case M: merge_sig => //=[S']; subst.
     move=> [??]; subst.
-    have {IH}/=[S[d' [H1 H2]]] := IH _ _ _ _ _ H dtA eA.
+    have {IH}/=[S[d' [H1 H2]]] := IH _ _ _ _ _ _ H MP dtA eA.
     have := same_ty_tc_tree_aux sP sV A' DA' (if has_cut A then maxD DA' DB else Pred).
     rewrite H2/= => /eqP.
     case Hz : tc_tree_aux => //=[[Dx sX]][?]; subst sX.
@@ -152,7 +174,8 @@ Proof.
     destruct DA'; simpl in *; subst => //.
     destruct DB => //=.
     congruence.
-  - move=> s INIT A sB B HINIT dA IH A' eA sV sV' r d ign H/=.
+    admit.
+  - move=> s INIT A sB B HINIT dA IH A' eA sV sV' sVx r d ign H/= MP.
     have [? fA] := expand_failed_same _ eA; subst A'.
     case: ifP => kA.
       move=> dtB <-/=; rewrite kA.
@@ -181,7 +204,7 @@ Proof.
     rewrite kA kB.
     repeat eexists; case:ifP => //=.
     rewrite failed_has_cut//=.
-  - move=> s INIT A sB B HINIT dA IH A' eA sV sV' r d ign H/=.
+  - move=> s INIT A sB B HINIT dA IH A' eA sV sV' sVx r d ign H/= MP.
     have [? sA]:= expand_solved_same _ eA; subst A'.
     rewrite success_is_ko//=.
     case: ifP => kB.
@@ -203,7 +226,7 @@ Proof.
     case M: merge_sig => //=[S'][??]; subst.
     rewrite success_is_ko// kB.
     repeat eexists.
-  - move=> s INIT A B0 B HINIT IH A' eA sV sV' r d ign H/= + <-/=.
+  - move=> s INIT A B0 B HINIT IH A' eA sV sV' sVx r d ign H/= MP + <-/=.
     have fA:= expand_not_failed _ eA notF.
     have sA:= expand_not_solved_not_success _ eA notF.
     rewrite failed_is_ko//=.
@@ -211,12 +234,12 @@ Proof.
     case dtB01: (tc_tree_aux _ _ B0) => /=[[DB01 sVB01]|]//=.
     case dtB1: (tc_tree_aux _ _ B) => /=[[DB1 sVB1]|]//=.
     case M: merge_sig => //=[S'][??]; subst.
-    have {IH}/=[S[d'[H1 H2]]] := IH _ _ _ _ _ H dtA1 eA.
+    have {IH}/=[S[d'[H1 H2]]] := IH _ _ _ _ _ _ H MP dtA1 eA.
     have:= same_ty_tc_tree_aux sP sV A' DA1 (maxD DB01 DB1).
     rewrite H2.
     case dtA1': (tc_tree_aux _ _ A') => /=[[DA1' sVA1']|]//=/eqP[?]; subst sVA1'.
     admit. (*TODO: pb with tc_tree_aux ran with a more precise subst then the hyp, should be solved using more_precise_tc_tree_aux *)
-  - move=> s INIT A B0 B HINIT IH A' eA sV sV' r d ign H/=.
+  - move=> s INIT A B0 B HINIT IH A' eA sV sV' sVx r d ign H/= MP.
     have fA:= expand_not_failed _ eA notF.
     rewrite failed_is_ko//=.
     case dtA: (tc_tree_aux _ _ A) => /=[[DA' sVA]|]//=.
@@ -225,7 +248,7 @@ Proof.
     case M: merge_sig => //=[S'][??]; subst.
     move=> <-{r}/=.
     admit. (*same as above...*)
-  - move=> s INIT A B0 B HINIT IH A' eA sV sV' r d ign H/=.
+  - move=> s INIT A B0 B HINIT IH A' eA sV sV' sVx r d ign H/= MP.
     have [? fA]:= expand_failed_same _ eA; subst A' => +<-{r}/=.
     case:ifP => kA.
       move=> [??]; subst; repeat eexists; rewrite minD_refl//.
@@ -254,7 +277,7 @@ Proof.
     have [[][//= _]] := tc_tree_aux_func2 dtA.
     rewrite dtA1 => -[?]; subst.
     destruct DB01 => /=;congruence.
-  - move=> s INIT A B0 B HINIT HL A' eA HR sV sV' r d ign H/= + <-{r}/=.
+  - move=> s INIT A B0 B HINIT HL A' eA HR sV sV' sVx r d ign H MP /= + <-{r}/=.
     have [? sA] := expand_solved_same _ eA; subst A'.
     rewrite success_is_ko//=.
     case dtA: (tc_tree_aux _ _ A) => /=[[DA' sVA]|]//=.
@@ -268,11 +291,37 @@ Proof.
       have:= same_ty_tc_tree_aux sP sVA B0 DA' DA1.
       rewrite dtB0/=.
       case dtB01: (tc_tree_aux _ _ B0) => /=[[DB01 sVB01]|]//=/eqP[?]; subst sVB01.
-      have:= HR _ _ _ _ _ _ dtB eB.
+      (* have: exists XX, sigma2ctx sP (get_substS s A) = Some XX /\ more_precise XX sVA.
+        admit.
+      move=> [XX [HH ZZ]].
+      have:= HR _ _ _ _ _ _ HH ZZ dtB eB.
+      move=> /=[S1[D1[Hx Hy]]].
+      have:= same_ty_tc_tree_aux sP sVA B' DB DA1.
+      rewrite Hy.
+      case dtB': tc_tree_aux => //=[[D S]]/eqP[?]; subst S.
+      have: exists T, merge_sig S1 sVB0 = ty_ok T by admit.
+      move=> [T H1]; rewrite H1; repeat eexists.
+      destruct DB0, DB; simpl in *; subst => //=.
+      have:= tc_tree_aux_func2 dtA.
+      rewrite dtA1/= => -[d2[H2 [?]]]; subst.
+      have:= tc_tree_aux_func2 dtB'.
+      rewrite Hy/= => -[d3[H3 [?]]]/=; subst.
+      simpl in *; subst.
+      have [d3[H4 H5]] := tc_tree_aux_func2 dtB01.
+      destruct d2; simpl in *; subst.
+        destruct D; try congruence.
+        destruct DB01, d3; try congruence.
+
+      destruct d3; simpl in *; subst => //=.
+      rewrite dtB0/= => -[d4[H4 [?]]]/=; subst.
+      simpl in *; subst.
+      destruct DB01 => //=.
+
+      rewrite Hy. *)
       admit. (*PB with ctx*)
     - have V := sigma2ctx_valid H.
-      rewrite cutl_tc_tree_aux// cutr_tc_tree_aux//=.
-      have /= := HR _ _ _ _ _ _ dtB eB.
+      rewrite cutl_tc_tree_aux//;[|admit]; rewrite cutr_tc_tree_aux//=; [|admit].
+      have /= := HR _ _ _ _ _ _ _ _ dtB eB.
       admit. (*PB with ctx*)
     - have [? fB] := expand_failed_same _ eB; subst B'.
       have:= same_ty_tc_tree_aux sP sV A ign (maxD DB0 DB).
@@ -334,10 +383,12 @@ Proof.
   - move=> s1 s2 A B sA _ <- sV sV' H1 H2.
     by have /=-> := success_det_tree_next_alt sA H2.
   - move=> s1 s2 r A B n eA _ IH sV sV' H1 dtA.
-    have /= [S' [d [<- H]]]:= expand_det_tree ckP H1 dtA eA; subst.
+    have V := sigma2ctx_valid H1.
+    have /= [S' [d [<- H]]]:= expand_det_tree ckP H1 (more_precise_refl V) dtA eA; subst.
     apply: IH (H1) H.
   - move=> s1 s2 r A B n eA _ IH sV sV' H1 dtA.
-    have /= [S' [d [<- H]]]:= expand_det_tree ckP H1 dtA eA; subst.
+    have V := sigma2ctx_valid H1.
+    have /= [S' [d [<- H]]]:= expand_det_tree ckP H1 (more_precise_refl V) dtA eA; subst.
     apply: IH (H1) H.
   - move=> s1 s2 A B r n fA nA _ IH sV sV' H1 H2.
     have V := sigma2ctx_valid H1.
